@prefix cs: <https://example.org/test_> .
@prefix dcat: <http://www.w3.org/ns/dcat#> .
@prefix dcterms: <http://purl.org/dc/terms/> .
@prefix owl: <http://www.w3.org/2002/07/owl#> .
@prefix skos: <http://www.w3.org/2004/02/skos/core#> .
@prefix xsd: <http://www.w3.org/2001/XMLSchema#> .

<https://example.org/col1> a skos:Collection ;
    dcterms:identifier "col1"^^xsd:token ;
    dcterms:isPartOf cs: ;
    dcterms:provenance "voc4cat-template"@en ;
    skos:definition "Collection of term related to linked data."@en ;
    skos:member <https://example.org/c01>,
        <https://example.org/c02>,
        <https://example.org/c03> ;
    skos:prefLabel "Linked data term"@en .

<https://example.org/c02> a skos:Concept ;
    dcterms:identifier "c02"^^xsd:token ;
    dcterms:provenance "https://www.w3.org/TR/2010/NOTE-curie-20101216/"@en ;
    skos:altLabel "CURIE"@en,
        "CompactURI"@en ;
    skos:broader <https://example.org/c01> ;
    skos:definition "A CURIE (or Compact URI) defines a generic, abbreviated syntax for expressing Uniform Resource Identifiers (URIs). "@en ;
    skos:inScheme cs: ;
    skos:prefLabel "Compact Universal Resource Locator"@en .

<https://example.org/c01> a skos:Concept ;
    dcterms:identifier "c01"^^xsd:token ;
    dcterms:provenance "https://datatracker.ietf.org/doc/html/rfc2396"@en ;
    skos:altLabel "URI"@en ;
    skos:definition "Uniform Resource Identifier is a compact string of characters for identifying an abstract or physical resource."@en ;
    skos:inScheme cs: ;
    skos:narrower <https://example.org/c02> ;
    skos:prefLabel "Uniform Resource Identifier"@en ;
    skos:relatedMatch <https://example.org/c03> ;
    skos:topConceptOf cs: .

<https://example.org/c03> a skos:Concept ;
    dcterms:identifier "c03"^^xsd:token ;
    dcterms:provenance "https://datatracker.ietf.org/doc/html/rfc3987"@en ;
    skos:altLabel "IRI"@en ;
    skos:definition "Internationalized Resource Identifier (IRI) is an internet protocol standard which builds on the Uniform Resource Identifier (URI) protocol by greatly expanding the set of permitted characters."@en ;
    skos:inScheme cs: ;
    skos:prefLabel "Internationalized Resource Identifier"@en ;
    skos:topConceptOf cs: .

cs: a skos:ConceptScheme ;
    dcterms:created "2023-03-10"^^xsd:date ;
    dcterms:creator <http://example.org/nfdi4cat/> ;
    dcterms:hasPart <https://example.org/col1> ;
    dcterms:identifier "test_"^^xsd:token ;
    dcterms:modified "2023-03-10"^^xsd:date ;
    dcterms:provenance "Sofia Garcia (orcid:0000-0001-2345-6789)"@en ;
    dcterms:publisher <http://example.org/nfdi4cat/> ;
    owl:versionInfo "v2023-03-10" ;
    skos:definition "A test vocabulary for the voc4cat template"@en ;
    skos:hasTopConcept <https://example.org/c01>,
        <https://example.org/c03> ;
    skos:prefLabel "Test-of-Voc4Cat"@en ;
    dcat:contactPoint "Sofia Garcia (orcid:0000-0001-2345-6789)" .

